WIP array iterator

src/cbor/raw/pulse/CBOR.Pulse.Raw.Read.fst
@@ -95,3 +95,270 @@ fn cbor_match_tagged_get_payload
   }
 }
 ```
+
+noeq
+type cbor_array_iterator =
+| CBOR_Array_Iterator_Slice:
+  s: Pulse.Lib.Slice.slice cbor_raw ->
+  slice_perm: perm ->
+  payload_perm: perm ->
+  cbor_array_iterator
+| CBOR_Array_Iterator_Serialized of cbor_serialized_array_iterator
+
+let cbor_array_iterator_slice_match
+  (pm: perm)
+  (slice_perm: perm)
+  (payload_perm: perm)
+  (s: Pulse.Lib.Slice.slice cbor_raw)
+  (l: list raw_data_item)
+: Tot slprop
+= exists* sq .
+     Pulse.Lib.Slice.pts_to s #(pm `perm_mul` slice_perm) sq **
+     PM.seq_list_match sq l (cbor_match (pm `perm_mul` payload_perm))
+
+let cbor_array_iterator_match
+  (pm: perm)
+  (i: cbor_array_iterator)
+  (l: list raw_data_item)
+: Tot slprop
+= match i with
+  | CBOR_Array_Iterator_Slice s slice_perm payload_perm ->
+    cbor_array_iterator_slice_match pm slice_perm payload_perm s l
+  | CBOR_Array_Iterator_Serialized s ->
+    cbor_serialized_array_iterator_match pm s l
+
+```pulse
+ghost
+fn cbor_match_array_elim
+  (c: cbor_array)
+  (p: perm)
+  (r: raw_data_item { Array? r })
+  requires
+    cbor_match_array c p r cbor_match
+  ensures exists* s . 
+    A.pts_to c.cbor_array_ptr #(p `perm_mul` c.cbor_array_array_perm) s **
+    PM.seq_list_match s (Array?.v r) (cbor_match (p `perm_mul` c.cbor_array_payload_perm)) **
+    trade
+      (A.pts_to c.cbor_array_ptr #(p `perm_mul` c.cbor_array_array_perm) s **
+        PM.seq_list_match s (Array?.v r) (cbor_match (p `perm_mul` c.cbor_array_payload_perm)))
+      (cbor_match_array c p r cbor_match) **
+    pure (c.cbor_array_length == Array?.len r)
+{
+  unfold (cbor_match_array c p r cbor_match);
+  with s . assert (A.pts_to c.cbor_array_ptr #(p `perm_mul` c.cbor_array_array_perm) s);
+  ghost
+  fn aux (_: unit)
+    requires emp ** (A.pts_to c.cbor_array_ptr #(p `perm_mul` c.cbor_array_array_perm) s **
+        PM.seq_list_match s (Array?.v r) (cbor_match (p `perm_mul` c.cbor_array_payload_perm)))
+    ensures cbor_match_array c p r cbor_match
+  {
+    fold (cbor_match_array c p r cbor_match)
+  };
+  Trade.intro _ _ _ aux
+}
+```
+
+#set-options "--print_implicits"
+
+```pulse
+ghost
+fn cbor_array_iterator_slice_match_intro
+  (c': cbor_array)
+  (pm: perm)
+  (s: Seq.seq cbor_raw)
+  (l: list raw_data_item)
+  (s': Pulse.Lib.Slice.slice cbor_raw)
+requires
+  A.pts_to c'.cbor_array_ptr #((pm `perm_mul` c'.cbor_array_array_perm) /. 2.0R) s **
+  Pulse.Lib.Slice.pts_to s' #((pm `perm_mul` c'.cbor_array_array_perm) /. 2.0R) s **
+  PM.seq_list_match s l (cbor_match (pm `perm_mul` c'.cbor_array_payload_perm)) **
+  Pulse.Lib.Slice.is_from_array c'.cbor_array_ptr ((pm `perm_mul` c'.cbor_array_array_perm) /. 2.0R) s'
+ensures
+  cbor_array_iterator_slice_match 1.0R ((pm `perm_mul` c'.cbor_array_array_perm) /. 2.0R) (pm `perm_mul` c'.cbor_array_payload_perm) s' l **
+  trade
+    (cbor_array_iterator_slice_match 1.0R ((pm `perm_mul` c'.cbor_array_array_perm) /. 2.0R) (pm `perm_mul` c'.cbor_array_payload_perm) s' l)
+    (A.pts_to c'.cbor_array_ptr #(pm `perm_mul` c'.cbor_array_array_perm) s **
+      PM.seq_list_match s l (cbor_match (pm `perm_mul` c'.cbor_array_payload_perm)))
+{
+  fold (cbor_array_iterator_slice_match 1.0R ((pm `perm_mul` c'.cbor_array_array_perm) /. 2.0R) (pm `perm_mul` c'.cbor_array_payload_perm) s' l);
+  ghost
+  fn aux (_: unit)
+    requires
+      (A.pts_to c'.cbor_array_ptr #((pm `perm_mul` c'.cbor_array_array_perm) /. 2.0R) s **
+        Pulse.Lib.Slice.is_from_array c'.cbor_array_ptr ((pm `perm_mul` c'.cbor_array_array_perm) /. 2.0R) s') **
+      cbor_array_iterator_slice_match 1.0R ((pm `perm_mul` c'.cbor_array_array_perm) /. 2.0R) (pm `perm_mul` c'.cbor_array_payload_perm) s' l
+    ensures
+      A.pts_to c'.cbor_array_ptr #(pm `perm_mul` c'.cbor_array_array_perm) s **
+      PM.seq_list_match s l (cbor_match (pm `perm_mul` c'.cbor_array_payload_perm))
+  {
+    unfold (cbor_array_iterator_slice_match 1.0R ((pm `perm_mul` c'.cbor_array_array_perm) /. 2.0R) (pm `perm_mul` c'.cbor_array_payload_perm) s' l);
+    Pulse.Lib.Slice.to_array s';
+    A.gather c'.cbor_array_ptr
+  };
+  Trade.intro _ _ _ aux
+}
+```
+  
+```pulse
+fn cbor_array_iterator_init
+  (c: cbor_raw)
+  (#pm: perm)
+  (#r: Ghost.erased raw_data_item { Array? r })
+requires
+    (cbor_match pm c r ** pure SZ.fits_u64)
+returns res: cbor_array_iterator
+ensures
+      cbor_array_iterator_match 1.0R res (Array?.v r) **
+      trade
+        (cbor_array_iterator_match 1.0R res (Array?.v r))
+        (cbor_match pm c r)
+{
+  cbor_match_cases c;
+  match c {
+    CBOR_Case_Serialized_Array c' -> {
+      Trade.rewrite_with_trade
+        (cbor_match pm c r)
+        (cbor_match_serialized_array c' pm r);
+      let i' = cbor_serialized_array_iterator_init c';
+      Trade.trans
+        (cbor_serialized_array_iterator_match 1.0R i' (Array?.v r))
+        (cbor_match_serialized_array c' pm r)
+        (cbor_match pm c r);
+      let i = CBOR_Array_Iterator_Serialized i';
+      Trade.rewrite_with_trade
+        (cbor_serialized_array_iterator_match 1.0R i' (Array?.v r))
+        (cbor_array_iterator_match 1.0R i (Array?.v r));
+      Trade.trans
+        (cbor_array_iterator_match 1.0R i (Array?.v r))
+        (cbor_serialized_array_iterator_match 1.0R i' (Array?.v r))
+        (cbor_match pm c r);
+      i
+    }
+    CBOR_Case_Array c' -> {
+      assert_norm (cbor_match pm (CBOR_Case_Array c') (Array (Array?.len r) (Array?.v r)) ==
+        cbor_match_array c' pm (Array (Array?.len r) (Array?.v r)) cbor_match
+      );
+      Trade.rewrite_with_trade
+        (cbor_match pm c r)
+        (cbor_match_array c' pm r cbor_match);
+      cbor_match_array_elim c' pm r;
+      with s . assert (A.pts_to c'.cbor_array_ptr #(pm `perm_mul` c'.cbor_array_array_perm) s);
+      Trade.trans
+        (A.pts_to c'.cbor_array_ptr #(pm `perm_mul` c'.cbor_array_array_perm) s **
+          PM.seq_list_match s (Array?.v r) (cbor_match (pm `perm_mul` c'.cbor_array_payload_perm)))
+        (cbor_match_array c' pm r cbor_match)
+        (cbor_match pm c r);
+      A.share c'.cbor_array_ptr;
+      let s' = Pulse.Lib.Slice.from_array false c'.cbor_array_ptr (SZ.uint64_to_sizet c'.cbor_array_length.value);
+      cbor_array_iterator_slice_match_intro _ _ _ _ _;
+      Trade.trans
+        (cbor_array_iterator_slice_match _ _ _ _ _)
+        _
+        (cbor_match pm c r);
+      let i = CBOR_Array_Iterator_Slice s' ((pm `perm_mul` c'.cbor_array_array_perm) /. 2.0R) (pm `perm_mul` c'.cbor_array_payload_perm);
+      Trade.rewrite_with_trade
+        (cbor_array_iterator_slice_match _ _ _ _ _)
+        (cbor_array_iterator_match 1.0R i (Array?.v r));
+      Trade.trans
+        (cbor_array_iterator_match 1.0R i (Array?.v r))
+        _
+        (cbor_match pm c r);
+      i
+    }
+  }
+}
+```
+
+```pulse
+fn cbor_array_iterator_is_empty
+  (c: cbor_array_iterator)
+  (#pm: perm)
+  (#r: Ghost.erased (list raw_data_item))
+requires
+    cbor_array_iterator_match pm c r
+returns res: bool
+ensures
+    cbor_array_iterator_match pm c r **
+    pure (res == Nil? r)
+{
+  match c {
+    CBOR_Array_Iterator_Serialized c' -> {
+      rewrite (cbor_array_iterator_match pm c r)
+        as (cbor_serialized_array_iterator_match pm c' r);
+      let res = cbor_serialized_array_iterator_is_empty c';
+      rewrite (cbor_serialized_array_iterator_match pm c' r)
+        as (cbor_array_iterator_match pm c r);
+      res
+    }
+    CBOR_Array_Iterator_Slice s ps pp -> {
+      rewrite (cbor_array_iterator_match pm c r)
+        as (cbor_array_iterator_slice_match pm ps pp s r);
+      unfold (cbor_array_iterator_slice_match pm ps pp s r);
+      PM.seq_list_match_length (cbor_match (pm `perm_mul` pp)) _ _;
+      Pulse.Lib.Slice.pts_to_len s;
+      let res = (Pulse.Lib.Slice.len s = 0sz);
+      fold (cbor_array_iterator_slice_match pm ps pp s r);
+      rewrite (cbor_array_iterator_slice_match pm ps pp s r)
+        as (cbor_array_iterator_match pm c r);
+      res
+    }
+  }
+}
+```
+
+```pulse
+fn cbor_array_iterator_next
+  (pi: R.ref cbor_array_iterator)
+  (#pm: perm)
+  (#i: Ghost.erased cbor_array_iterator)
+  (#l: Ghost.erased (list raw_data_item))
+requires
+    R.pts_to pi i **
+    cbor_array_iterator_match pm i l **
+    pure (Cons? l)
+returns res: cbor_raw
+ensures exists* a p i' q .
+    cbor_match p res a **
+    R.pts_to pi i' **
+    cbor_array_iterator_match pm i' q **
+    trade
+      (cbor_match p res a ** cbor_array_iterator_match pm i' q)
+      (cbor_array_iterator_match pm i l) **
+    pure (Ghost.reveal l == a :: q)
+{
+  let i = !pi;
+  match i {
+    CBOR_Array_Iterator_Serialized i_ -> {
+      let mut pi_ = i_;
+      Trade.rewrite_with_trade (cbor_array_iterator_match pm i l)
+        (cbor_serialized_array_iterator_match pm i_ l);
+      let res = cbor_serialized_array_iterator_next pi_;
+      let i'_ = !pi_;
+      with q . assert (cbor_serialized_array_iterator_match pm i'_ q);
+      let i' = CBOR_Array_Iterator_Serialized i'_;
+      Trade.rewrite_with_trade
+        (cbor_serialized_array_iterator_match pm i'_ q)
+        (cbor_array_iterator_match pm i' q);
+      with p a . assert (cbor_match p res a);
+      Trade.reg_l
+        (cbor_match p res a)
+        (cbor_array_iterator_match pm i' q)
+        (cbor_serialized_array_iterator_match pm i'_ q);
+      Trade.trans
+        (cbor_match p res a ** cbor_array_iterator_match pm i' q)
+        (cbor_match p res a ** cbor_serialized_array_iterator_match pm i'_ q)
+        (cbor_serialized_array_iterator_match pm i_ l);
+      Trade.trans
+        (cbor_match p res a ** cbor_array_iterator_match pm i' q)
+        (cbor_serialized_array_iterator_match pm i_ l)
+        (cbor_array_iterator_match pm i l);
+      pi := i';
+      res
+    }
+    CBOR_Array_Iterator_Slice s ps pp -> {
+      admit ()
+    }
+  }
+}
+```
+
