src/cbor/raw/pulse/CBOR.Pulse.Raw.Serialized.fsti
@@ -23,3 +23,54 @@ val cbor_match_serialized_tagged_get_payload
       (cbor_match 1.0R res (Tagged?.v r))
       (cbor_match_serialized_tagged c pm r)
   )
+
+[@@CAbstractStruct]
+val cbor_serialized_array_iterator: Type0
+
+val cbor_serialized_array_iterator_match
+  (p: perm)
+  (i: cbor_serialized_array_iterator)
+  (a: list raw_data_item)
+: slprop
+
+val cbor_serialized_array_iterator_init
+  (c: cbor_serialized)
+  (#pm: perm)
+  (#r: Ghost.erased raw_data_item { Array? r })
+: stt cbor_serialized_array_iterator
+    (cbor_match_serialized_array c pm r)
+    (fun res ->
+      cbor_serialized_array_iterator_match 1.0R res (Array?.v r) **
+      trade
+        (cbor_serialized_array_iterator_match 1.0R res (Array?.v r))
+        (cbor_match_serialized_array c pm r)
+    )
+
+val cbor_serialized_array_iterator_is_empty
+  (i: cbor_serialized_array_iterator)
+  (#pm: perm)
+  (#l: Ghost.erased (list raw_data_item))
+: stt bool
+  (cbor_serialized_array_iterator_match pm i l)
+  (fun res ->
+    cbor_serialized_array_iterator_match pm i l **
+    pure (res == Nil? l)
+  )
+
+val cbor_serialized_array_iterator_next
+  (pi: ref cbor_serialized_array_iterator)
+  (#pm: perm)
+  (#i: Ghost.erased cbor_serialized_array_iterator)
+  (#l: Ghost.erased (list raw_data_item))
+: stt cbor_raw
+  (pts_to pi i ** cbor_serialized_array_iterator_match pm i l ** pure (Cons? l))
+  (fun res -> exists* a i' q .
+    pts_to pi i' **
+    cbor_match pm res a **
+    cbor_serialized_array_iterator_match pm i' q **
+    trade
+      (cbor_match pm res a **
+        cbor_serialized_array_iterator_match pm i' q)
+      (cbor_serialized_array_iterator_match pm i l) **
+    pure (Ghost.reveal l == a :: q)
+  )
